Lemma lem_mmLR_sumForm qed

test/testMasterM2.dfy
@@ -1,5 +1,5 @@
 
-include "../theory/masterM.dfy"
+include "../theory/masterLR.dfy"
 
 // Recurrence:
 //   T1(n) = / 0             , n <= 0
@@ -36,9 +36,9 @@ lemma test_masterMethodForT1lifted()
 
   assert b >= s-1;  
   forall n:nat 
-    ensures T1'(n) == TbodyLR2(a, b, c, s, T1', w, n)
+    ensures T1'(n) == TbodyLR(a, b, c, s, T1', w, n)
   {
-    reveal TbodyLR2;
+    reveal TbodyLR;
     lem_T1def(n);
   }           
   assert bigOR0(w, n => powr(n as R0, k)) by {   
@@ -53,7 +53,7 @@ lemma test_masterMethodForT1lifted()
     }
     assert bigOR0from(1.0, 1, w, polyGrowthR0(k));
   } 
-  masterMethodLR2(a, b, c, s, T1', w, k);
+  thm_masterMethodLR(a, b, c, s, T1', w, k);
 }   
 
 //**************************************************************************//
@@ -93,9 +93,9 @@ lemma test_masterMethodForT2lifted()
 
   assert b >= s-1;  
   forall n:nat 
-    ensures T2'(n) == TbodyLR2(a, b, c, s, T2', w, n)
+    ensures T2'(n) == TbodyLR(a, b, c, s, T2', w, n)
   {
-    reveal TbodyLR2;
+    reveal TbodyLR;
     lem_T2def(n);
   }
   assert bigOR0(w, n => powr(n as R0, k)) by {  // k=0
@@ -110,5 +110,62 @@ lemma test_masterMethodForT2lifted()
     }
     assert bigOR0from(1.0, 1, w, polyGrowthR0(k));
   } 
-  masterMethodLR2(a, b, c, s, T2', w, k); 
+  thm_masterMethodLR(a, b, c, s, T2', w, k); 
+} 
+
+//**************************************************************************//
+
+// Recurrence:
+//   T3(n) = / 0             , n <= 4
+//           \ T3(n-1) + 1   , n > 4
+opaque ghost function T3(n:nat) : nat
+  decreases n
+{
+  if n <= 4
+  then 0  
+  else T3(n-1) + 1 
+}
+
+lemma lem_T3def(n:nat)
+  ensures n <= 4 ==> T3(n) == 0
+  ensures n > 4  ==> T3(n) == 1*T3(n-1) + 1
+{
+  reveal T3();
+}
+
+// Exact closed form:
+//   T2(n) = 1/4*(2*n - (-1)^n - (-1)^(2 n) - 2)
+// Asymptotic closed form:
+//   T2(n) in O(n)
+lemma test_masterMethodForT3lifted() 
+  ensures bigOR0(liftToR0(T3), n => powr(n as R0, 1.0))
+{
+  var a:nat       := 1;
+  var b:nat       := 4;
+  var c:R0        := 0.0;
+  var s:nat       := 1;
+  var k:R0        := 0.0;
+  var T3':nat->R0 := liftToR0(T3);
+  var w:nat->R0   := liftToR0(n => 1);
+
+  assert b >= s-1;  
+  forall n:nat 
+    ensures T3'(n) == TbodyLR(a, b, c, s, T3', w, n)
+  {
+    reveal TbodyLR;
+    lem_T3def(n);
+  }
+  assert bigOR0(w, n => powr(n as R0, k)) by {  // k=0
+    // we show that c=1 and n0=1
+    forall n:nat 
+      ensures 0 <= 1 <= n ==> w(n) <= 1.0*polyGrowthR0(k)(n)
+    {
+      if 0 <= 1 <= n {
+        assert polyGrowthR0(k)(n) == 1.0 by { lem_powrZeroAll(); }
+        assert 1.0 <= 1.0*polyGrowthR0(k)(n); 
+      }
+    }
+    assert bigOR0from(1.0, 1, w, polyGrowthR0(k));
+  } 
+  thm_masterMethodLR(a, b, c, s, T3', w, k); 
 } 
