analysisByMM/quadTriangle.dfy
@@ -1,8 +1,8 @@
 
 include "../theory/complexity.dfy"
-include "../theory/masterM.dfy"
+include "../theory/masterLR.dfy"
 
-method quadTriangle(N:nat) 
+method quadTriangle(N:nat)
   returns (ghost t:nat, ghost t':nat)
   ensures t == T1(N)
   ensures bigOR0(liftToR0(T1), n => powr(n as R0, 2.0))
@@ -74,15 +74,15 @@ lemma lem_T1BigOquad()
 
   assert b >= s-1;
   forall n:nat 
-    ensures T1'(n) == TbodyLR2(a, b, c, s, T1', w, n)
+    ensures T1'(n) == TbodyLR(a, b, c, s, T1', w, n)
   {
-    reveal TbodyLR2; 
+    reveal TbodyLR; 
     lem_T1def(n);
   } 
   assert bigOR0(w, n => powr(n as R0, k)) by {   
     lem_T2BigOlin();
   } 
-  masterMethodLR2(a, b, c, s, T1', w, k);
+  thm_masterMethodLR(a, b, c, s, T1', w, k);
 }
 
 lemma lem_T2BigOlin()
@@ -98,9 +98,9 @@ lemma lem_T2BigOlin()
 
   assert b >= s-1;  
   forall n:nat 
-    ensures T2'(n) == TbodyLR2(a, b, c, s, T2', w, n)
+    ensures T2'(n) == TbodyLR(a, b, c, s, T2', w, n)
   {
-    reveal TbodyLR2;
+    reveal TbodyLR;
     lem_T2def(n);
   }  
   assert bigOR0(w, n => powr(n as R0, k)) by {   
@@ -113,5 +113,5 @@ lemma lem_T2BigOlin()
     }
     assert bigOR0from(1.0, 1, w, polyGrowthR0(k));
   } 
-  masterMethodLR2(a, b, c, s, T2', w, k);
+  thm_masterMethodLR(a, b, c, s, T2', w, k);
 }
