theory/masterLR.dfy
@@ -1,0 +1,403 @@
+
+include "./complexity.dfy"
+
+// Following recurrence models a recursive computation where
+//      a = Branching factor, or number of recursive calls. Controls the breadth of computation.
+//      b = Base case condition.
+//      s = Step Size. Controls the depth of computation.
+//      c = Cost at the base case
+//   w(n) = Additive term, cost by recursive call.
+//
+//  It is assumed sub-exponential work is donde at each recursive call
+//  (if not we would be doing exponential work from the very beggining!).
+//
+// Let T:nat->R0 be such that
+//   T(n) = / c                 , n <= b        
+//          \ a*T(n-s) + w(n)   , n > b           
+// where a>0, s>0, b >= s-1 and w in O(n^k) for some k.    
+// Then:
+//   T(n) = / O(n^{k+1})        , a = 1
+//          \ O(n^k*a^{n/s})    , a > 1
+//
+// Note. Always match w to the tightest Θ(n^k) it belongs. 
+//       - It is neccesary and sufficient to conclude the 
+//         thight Θ(n^{k+1}) bound when a=1.
+//       - It is neccesary, but not always sufficient, to conclude the 
+//         thight Θ(n^k*a^{n/s}) bound when a>1.
+//       In general, we can only be sure of O type bounds. Thigher Θ bounds
+//       require a case by case analysis.
+lemma {:axiom} thm_masterMethodLR(a:nat, b:nat, c:R0, s:nat, T:nat->R0, w:nat->R0, k:R0)  
+  requires a > 0 && s > 0 && b >= s-1
+  requires bigOR0(w, n => powr(n as R0, k)) 
+  requires forall n:nat :: T(n) == TbodyLR(a, b, c, s, T, w, n) 
+
+  ensures a == 1 ==> bigOR0(T, (n:nat) => powr(n as R0, k + 1.0))
+  ensures a > 1  ==> bigOR0(T, (n:nat) => powr(n as R0, k)*powr(a as R0, (n/s) as R0))
+{
+  // 1. Prove: ∀ n : T(n) = a^m*c + S(n) where m=ceil((n-b)/s)
+  assert forall n:nat :: T(n) == TsumForm(a, b, c, s, w, n)
+    by { lem_mmLR_sumForm(a, b, c, s, T, w); }
+
+  // 2. Prove: ∃ d: ∀ n : S(n) <= d*n^k*sum_{i=0}^{m-1}a^i
+  assert exists d :: SupBoundPred(a, b, s, w, k, d)
+    by { lem_mmLR_SupBound(a, b, c, s, T, w, k); }
+
+  // Cases on a:
+  if a == 1 {    
+//     assert sumr(0, m-1, i => powr(a as R0, i as real)) == m;
+//     assert bigOR0(n => m, n => powr(n as R0, 1.0));
+//
+//     assert bigOR0(T, (n:nat) => powr(n as R0, k + 1.0));
+  } else if a > 1 {
+//     assert sumr(0, m-1, i => powr(a as R0, i as real)) == ...;
+//     assert bigOR0(n => ..., n => powr(a as R0, (n/s) as R0));
+//      
+//     assert bigOR0(T, (n:nat) => powr(n as R0, k)*powr(a as R0, (n/s) as R0));
+  }
+  assert false;
+}
+
+opaque ghost function TbodyLR(a:nat, b:nat, c:R0, s:nat, T:nat->R0, w:nat->R0, n:nat) : R0
+  requires b >= s-1
+{    
+  if   n <= b 
+  then c
+  else (a as R0)*T(n - s) + w(n)    
+} 
+
+// Expression: ceil((n-b)/s)
+opaque ghost function m(b:nat, s:nat, n:nat) : int
+  requires s > 0
+{    
+  max(0, ceil(((n-b) as real)/(s as real)))  
+} 
+
+// Expression: a^m*c + S(n)
+opaque ghost function TsumForm(a:nat, b:nat, c:R0, s:nat, w:nat->R0, n:nat) : real
+  requires s > 0
+{    
+  powr(a as R0, m(b,s,n) as real)*c + S(a, b, s, w, n)    
+} 
+
+// Expression: sum_{i=0}^{m-1}a^i*w(n-i*s)
+opaque ghost function S(a:nat, b:nat, s:nat, w:nat->R0, n:nat) : real
+  requires s > 0
+{    
+  sumr(0, m(b,s,n)-1, i => S1(a,i)*S2(s,w,n,i))      
+} 
+
+// Expression: a^i
+opaque ghost function S1(a:nat, i:int) : real
+{    
+  powr(a as R0, i as real)     
+} 
+
+// Expression: n-i*s
+opaque ghost function S2(s:nat, w:nat->R0, n:nat, i:int) : real
+{    
+  liftD(w,0.0)(n-i*s)
+} 
+
+// Expression: d*n^k*sum_{i=0}^{m-1}a^i
+opaque ghost function SupBound(a:nat, b:nat, s:nat, w:nat->R0, k:R0, n:nat, d:R0) : real
+  requires s > 0
+{    
+  d*powr(n as R0, k)*sumr(0, m(b,s,n)-1, i => S1(a,i))    
+} 
+
+// Predicate: ∀ n : S(n) <= SupBound(n,d)
+ghost predicate SupBoundPred(a:nat, b:nat, s:nat, w:nat->R0, k:R0, d:R0)
+  requires s > 0
+{    
+  forall n:nat :: S(a, b, s, w, n) <= SupBound(a, b, s, w, k, n, d) 
+} 
+
+// If n <= b then m = 0
+// If n > b  then m = ceil((n-b)/s)
+lemma lem_mmLR_mValue(b:nat, s:nat, n:nat)  
+  requires s > 0 && b >= s-1
+  ensures  n <= b ==> m(b,s,n) == 0
+  ensures  n >  b ==> m(b,s,n) == ceil(((n-b) as real)/(s as real))
+                      && m(b,s,n) >= 1
+{
+  if n <= b {
+    calc {  // ceil((n-b)/s) <= 0
+         ceil(((n-b) as real)/(s as real));
+      <= { assert ((n-b) as real)/(s as real) <= 0.0; 
+           lem_ceilxLEQnIFFxLEQn(((n-b) as real)/(s as real),0); }
+         0;
+    }  
+    calc {
+         m(b,s,n);
+      == { reveal m(); }
+         max(0, ceil(((n-b) as real)/(s as real)));
+      == max(0, 0);
+      == 0;
+    }  
+  } else if n > b {
+    calc {  // ceil((n-b)/s) > 0
+        ceil(((n-b) as real)/(s as real));
+      > { assert ((n-b) as real)/(s as real) > 0.0; 
+          lem_ceilxLEQnIFFxLEQn(((n-b) as real)/(s as real),0); }
+        0;
+    }  
+    calc {
+         m(b,s,n);
+      == { reveal m(); }
+         max(0, ceil(((n-b) as real)/(s as real)));
+      == ceil(((n-b) as real)/(s as real));
+    }  
+  }
+}
+
+// ∀ n : T(n) = a^m*c + sum_{i=0}^{m-1}a^i*w(n-i*s) where m=ceil((n-b)/s)
+lemma lem_mmLR_sumForm(a:nat, b:nat, c:R0, s:nat, T:nat->R0, w:nat->R0)  
+  requires a > 0 && s > 0 && b >= s-1
+  requires forall n:nat :: T(n) == TbodyLR(a, b, c, s, T, w, n) 
+  ensures  forall n:nat :: T(n) == TsumForm(a, b, c, s, w, n)     
+{
+  forall n:nat
+    ensures T(n) == TsumForm(a, b, c, s, w, n)
+  {
+    lem_mmLR_sumFormInd(a, b, c, s, T, w, n);
+  }
+}
+
+lemma lem_mmLR_sumFormInd(a:nat, b:nat, c:R0, s:nat, T:nat->R0, w:nat->R0, n:nat)  
+  requires a > 0 && s > 0 && b >= s-1
+  requires forall n:nat :: T(n) == TbodyLR(a, b, c, s, T, w, n)  
+  ensures  T(n) == TsumForm(a, b, c, s, w, n)    
+{
+  var mv := m(b,s,n);
+  var aR := a as R0; 
+  if n <= b {
+    // CB. n <= b
+    calc {
+         T(n);
+      == { reveal TbodyLR(); }
+         c;
+      == { lem_mmLR_mValue(b, s, n); reveal S, sumr();  }
+         c + S(a, b, s, w, n);
+      == { lem_mmLR_mValue(b, s, n); lem_powrZero(aR); }
+         powr(aR, mv as real)*c + S(a, b, s, w, n);
+      == { reveal TsumForm(); } 
+         TsumForm(a, b, c, s, w, n);  
+    }      
+  } else {
+    // Step. n > b
+    //   IH: T(n-s) = TsumForm(a, b, c, s, w, n-s)   
+    //    T: T(n)   = TsumForm(a, b, c, s, w, n)   
+    var mv' := m(b,s,n-s);
+    assert mv >= 1 by { lem_mmLR_mValue(b, s, n); }
+
+    // First, we prove various named rewritings that will be used in the final proof
+    assert mRewr: mv' == mv - 1 
+      by { lem_mmLR_mRewr(a,b,s,n); }
+    assert sumRewr:    S(a, b, s, w, n-s) 
+                    == sumr(0, mv-2, i => S1(a,i)*S2(s,w,n,i+1))
+      by { lem_mmLR_sumRewr(a, b, c, s, T, w, n); }
+    assert sumRewr2:    aR*sumr(0, mv-2, i => S1(a,i)*S2(s,w,n,i+1))
+                     == sumr(0, mv-2, i => S1(a,i+1)*S2(s,w,n,i+1))
+      by { lem_mmLR_sumRewr2(a, b, c, s, T, w, n); }  
+    assert sumRewr3:    sumr(0, mv-2, i => S1(a,i+1)*S2(s,w,n,i+1))  
+                     == sumr(1, mv-1, i => S1(a,i)*S2(s,w,n,i))
+      by { lem_mmLR_sumRewr3(a, b, c, s, T, w, n); }
+    assert wRewr: w(n) == S1(a,0)*S2(s,w,n,0)
+      by {
+        calc {
+             S1(a,0)*S2(s,w,n,0);
+          == { reveal S2(); } 
+             S1(a,0)*liftD(w,0.0)(n-0*s);
+          == { reveal S1(); } 
+             powr(a as R0, 0 as real)*liftD(w,0.0)(n-0*s); 
+          == { lem_powrZero(a as R0); }    
+             1.0*liftD(w,0.0)(n-0*s); 
+          == { lem_powrZero(a as R0); }    
+             liftD(w,0.0)(n);             
+        }      
+      }  
+
+    // Finally, we prove the desired goal
+    calc {
+         T(n);
+      == { reveal TbodyLR(); assert n > b; }
+         aR*T(n - s) + w(n); 
+      == { lem_mmLR_sumFormInd(a, b, c, s, T, w, n-s); }
+         aR*TsumForm(a, b, c, s, w, n-s) + w(n); 
+      == { reveal TsumForm(); }
+         aR*(powr(aR, mv' as real)*c + S(a, b, s, w, n-s)) + w(n);  
+      == { reveal mRewr; }
+         aR*(powr(aR, (mv-1) as real)*c + S(a, b, s, w, n-s)) + w(n); 
+      == aR*powr(aR, (mv-1) as real)*c + aR*S(a, b, s, w, n-s) + w(n); 
+      == { lem_powrDef(aR, (mv-1) as real); }
+         powr(aR, mv as real)*c + aR*S(a, b, s, w, n-s) + w(n);     
+      == { reveal sumRewr; }
+         powr(aR, mv as real)*c + aR*sumr(0, mv-2, i => S1(a,i)*S2(s,w,n,i+1)) + w(n);
+      == { reveal sumRewr2; }
+         powr(aR, mv as real)*c + sumr(0, mv-2, i => S1(a,i+1)*S2(s,w,n,i+1)) + w(n);    
+      == { reveal sumRewr3; }
+         powr(aR, mv as real)*c + sumr(1, mv-1, i => S1(a,i)*S2(s,w,n,i)) + w(n); 
+      == { reveal wRewr; }
+         powr(aR, mv as real)*c + sumr(1, mv-1, i => S1(a,i)*S2(s,w,n,i)) + S1(a,0)*S2(s,w,n,0); 
+      == { reveal sumr(); }
+         powr(aR, mv as real)*c + sumr(0, mv-1, i => S1(a,i)*S2(s,w,n,i));           
+      == { reveal TsumForm(), S(); }
+         TsumForm(a, b, c, s, w, n);                                                                   
+    }  
+  } 
+}
+
+lemma lem_mmLR_sumRewr3(a:nat, b:nat, c:R0, s:nat, T:nat->R0, w:nat->R0, n:nat)  
+  requires a > 0 && s > 0 && b >= s-1
+  requires n > b
+  requires m(b,s,n) >= 1
+  ensures     sumr(0, m(b,s,n)-2, i => S1(a,i+1)*S2(s,w,n,i+1))  
+           == sumr(1, m(b,s,n)-1, i => S1(a,i)*S2(s,w,n,i))
+{
+  var mv := m(b,s,n); assert mv >= 1;
+  calc {
+        sumr(0, mv-2, i => S1(a,i+1)*S2(s,w,n,i+1));
+    == { lem_sumr_shiftIndex(0, mv-2, 1, i => S1(a,i+1)*S2(s,w,n,i+1)); } 
+        sumr(1, mv-1, l => (i => S1(a,i+1)*S2(s,w,n,i+1))(l-1)); 
+    == { reveal S2();
+          assert forall l :: 1 <= l <= mv-1 ==> 
+            (i => S1(a,i+1)*S2(s,w,n,i+1))(l-1) == S1(a,l)*S2(s,w,n,l);
+          lem_sumr_leibniz(1, mv-1, l => (i => S1(a,i+1)*S2(s,w,n,i+1))(l-1), 
+                                    l => S1(a,l)*S2(s,w,n,l)); } 
+        sumr(1, mv-1, i => S1(a,i)*S2(s,w,n,i));            
+  }      
+}
+
+lemma {:isolate_assertions} lem_mmLR_sumRewr2(a:nat, b:nat, c:R0, s:nat, T:nat->R0, w:nat->R0, n:nat)  
+  requires a > 0 && s > 0 && b >= s-1
+  requires n > b
+  requires m(b,s,n) >= 1
+  ensures    (a as R0)*sumr(0, m(b,s,n)-2, i => S1(a,i)*S2(s,w,n,i+1))
+          == sumr(0, m(b,s,n)-2, i => S1(a,i+1)*S2(s,w,n,i+1))
+{
+  var mv := m(b,s,n); assert mv >= 1;
+  var aR := a as R0;
+    calc {
+          aR*sumr(0, mv-2, i => S1(a,i)*S2(s,w,n,i+1));
+      == { lem_sumr_linearityConst(0, mv-2, aR, i => S1(a,i)*S2(s,w,n,i+1)); }
+          sumr(0, mv-2, l => aR*(i => S1(a,i)*S2(s,w,n,i+1))(l)); 
+      == { reveal S1(); assert aR == a as real;
+           assert forall l :: 
+              0 <= l <= mv-2 ==> 
+                aR*(i => S1(a,i)*S2(s,w,n,i+1))(l) 
+                == aR*powr(a as real,l as real)*S2(s,w,n,l+1);
+           lem_sumr_leibniz(0, mv-2, l => aR*(i => S1(a,i)*S2(s,w,n,i+1))(l), 
+                                     l => aR*powr(a as real,l as real)*S2(s,w,n,l+1)); } 
+          sumr(0, mv-2, i => aR*powr(aR,i as real)*S2(s,w,n,i+1));  
+      == { reveal S1(); lem_powrDefAll();
+           assert forall l :: 0 <= l <= mv-2 ==> 
+              aR*powr(aR,l as real)*S2(s,w,n,l+1) == S1(a,l+1)*S2(s,w,n,l+1);
+           lem_sumr_leibniz(0, mv-2, i => aR*powr(aR,i as real)*S2(s,w,n,i+1), 
+                                     i => S1(a,i+1)*S2(s,w,n,i+1)); }       
+          sumr(0, mv-2, i => S1(a,i+1)*S2(s,w,n,i+1));       
+    }         
+}
+
+lemma lem_mmLR_sumRewr(a:nat, b:nat, c:R0, s:nat, T:nat->R0, w:nat->R0, n:nat)  
+  requires a > 0 && s > 0 && b >= s-1
+  requires n > b
+  requires m(b,s,n) >= 1
+  ensures S(a, b, s, w, n-s) == sumr(0, m(b,s,n)-2, i => S1(a,i)*S2(s,w,n,i+1))
+{
+  var mv := m(b,s,n); assert mv >= 1;
+  calc { 
+        S(a, b, s, w, n-s);
+    == { reveal S(); lem_mmLR_mRewr(a, b, s, n); }
+        sumr(0, mv-2, i => S1(a,i)*S2(s,w,n-s,i));
+    == { reveal S2();
+          assert forall i :: 0 <= i <= mv-2 ==> 
+            S1(a,i)*S2(s,w,n-s,i) == S1(a,i)*liftD(w,0.0)((n-s)-i*s);
+          lem_sumr_leibniz(0, mv-2, i => S1(a,i)*S2(s,w,n-s,i), 
+                                    i => S1(a,i)*liftD(w,0.0)((n-s)-i*s));  }
+       sumr(0, mv-2, i => S1(a,i)*liftD(w,0.0)((n-s)-i*s)); 
+    == { assert forall i {:trigger S1(a,i), liftD(w,0.0)((n-s)-i*s)} :: 
+            0 <= i <= mv-2 ==>     S1(a,i)*liftD(w,0.0)((n-s)-i*s) 
+                                == S1(a,i)*liftD(w,0.0)(n-(i+1)*s);
+          lem_sumr_leibniz(0, mv-2, i => S1(a,i)*liftD(w,0.0)((n-s)-i*s), 
+                                    i => S1(a,i)*liftD(w,0.0)(n-(i+1)*s));  }
+       sumr(0, mv-2, i => S1(a,i)*liftD(w,0.0)((n-(i+1)*s)));  
+    == { reveal S2();
+          assert forall i :: 0 <= i <= mv-2 ==> 
+            S1(a,i)*liftD(w,0.0)(n-(i+1)*s) == S1(a,i)*S2(s,w,n,i+1);
+          lem_sumr_leibniz(0, mv-2, i => S1(a,i)*liftD(w,0.0)(n-(i+1)*s), 
+                                    i => S1(a,i)*S2(s,w,n,i+1));  }
+       sumr(0, mv-2, i => S1(a,i)*S2(s,w,n,i+1));      
+  }  
+}
+
+// m = m' - 1
+// ceil(((n-s)-b)/s) = m=ceil((n-b)/s) - 1
+lemma lem_mmLR_mRewr(a:nat, b:nat, s:nat, n:nat)  
+  requires a > 0 && s > 0 && b >= s-1
+  requires n > b
+  requires m(b,s,n) >= 1
+  ensures  m(b,s,n-s) == m(b,s,n) - 1
+{
+  assert arith:   (((n-b)-s) as real)/(s as real) 
+               == ((((n-b) as real)/(s as real)) - ((s/s) as real));
+  calc {
+       m(b,s,n-s);
+    == { reveal m(); }
+       max(0, ceil((((n-s)-b) as real)/(s as real)));
+    == max(0, ceil((((n-b)-s) as real)/(s as real))); 
+    == { reveal arith; }
+       max(0, ceil(((((n-b) as real)/(s as real)) - ((s/s) as real)) as real));
+    == max(0, ceil(((n-b) as real)/(s as real)) - 1);
+    == { assert ceil(((n-b) as real)/(s as real)) - 1 >= 0; } 
+       ceil(((n-b) as real)/(s as real)) - 1;
+    == { assert ceil(((n-b) as real)/(s as real)) > 0; }
+       max(0, ceil(((n-b) as real)/(s as real))) - 1;  
+    == { reveal m(); }
+       m(b,s,n) - 1;    
+  }  
+}
+
+// ∃ d: ∀ n : S(n) <= Sbound(n,d)
+// ∃ d: ∀ n : S(n) <= d*n^k*sum_{i=0}^{m-1}a^i
+lemma {:axiom} lem_mmLR_SupBound(a:nat, b:nat, c:R0, s:nat, T:nat->R0, w:nat->R0, k:R0)  
+  requires a > 0 && s > 0 && b >= s-1
+  requires bigOR0(w, n => powr(n as R0, k))
+  ensures exists d :: SupBoundPred(a, b, s, w, k, d)
+
+
+// A special case of thm_masterMethodLR.
+// This version doesn't admit recurrences with base case at n <= 0.
+//
+// Let T:nat->R0 be such that
+//   T(n) = / c                 , n <= b        
+//          \ a*T(n-b) + w(n)   , n > b           
+// where a>0, b>0 and w in O(n^k) for some k.    
+// Then:
+//   T(n) = / O(n^{k+1})        , a = 1
+//          \ O(n^k*a^{n/b})    , a > 1
+lemma thm_masterMethodLR2(a:nat, b:nat, c:R0, T:nat->R0, w:nat->R0, k:R0)  
+  requires a > 0 && b > 0
+  requires bigOR0(w, (n:nat) => powr(n as R0, k)) 
+  requires forall n:nat :: T(n) == TbodyLR2(a, b, c, T, w, n) 
+
+  ensures a == 1 ==> bigOR0(T, (n:nat) => powr(n as R0, k + 1.0))
+  ensures a > 1  ==> bigOR0(T, (n:nat) => powr(n as R0, k)*powr(a as R0, (n/b) as R0))
+{
+  // proof using thm_masterMethodLR with s := b.
+  assert a > 0;   
+  assert b > 0;   
+  assert b >= b - 1;
+  assert bigOR0(w, n => powr(n as R0, k));
+  assert forall n:nat :: T(n) == TbodyLR2(a, b, c, T, w, n); 
+  assert forall n:nat :: T(n) == TbodyLR(a, b, c, b, T, w, n)
+    by { reveal TbodyLR2, TbodyLR; } 
+
+  thm_masterMethodLR(a, b, c, b, T, w, k);
+}
+
+opaque ghost function TbodyLR2(a:nat, b:nat, c:R0, T:nat->R0, w:nat->R0, n:nat) : R0
+{   
+  if   n <= b 
+  then c
+  else (a as R0)*T(n - b) + w(n)   
+} 
